iodiv/IODiv.fst
@@ -1,0 +1,486 @@
+module IODiv
+
+open FStar.List.Tot
+open FStar.List.Tot.Properties
+open FStar.Classical
+open FStar.IndefiniteDescription
+open FStar.Calc
+open Util
+open Itree
+
+(** IODiv
+
+    In this file we define a more complete version of the IODiv effect for I/O and
+    non-termination than in SIODiv.
+
+*)
+
+(** Monad instance
+
+   Without GetTrace for now
+
+*)
+
+assume val file_descr : eqtype
+
+type cmds = | Openfile | Read | Close
+
+unfold let io_args cmd : eqtype =
+  match cmd with
+  | Openfile -> string
+  | Read -> file_descr
+  | Close -> file_descr
+
+unfold let io_res cmd : eqtype =
+  match cmd with
+  | Openfile -> file_descr
+  | Read -> string
+  | Close -> unit
+
+let io_op_sig : op_sig cmds = {
+  args = io_args ;
+  res = io_res
+}
+
+unfold
+let iotree a = itree cmds io_op_sig a
+
+unfold
+let iopos = ipos cmds io_op_sig
+
+unfold
+let iochoice = ichoice cmds io_op_sig
+
+unfold
+let iopostream = postream cmds io_op_sig
+
+unfold
+let ioret #a (x : a) : iotree a =
+  ret x
+
+(**
+  Spec with trace
+  The trace contains the response of the environment, in fact it is a subset of
+  positions where Tau steps are ignored.
+
+  For non-termination however, we make use of potentially infinite traces.
+*)
+
+let trace = list (c: iochoice { c <> Tau_choice })
+
+let rec ipos_trace (p : iopos) : trace =
+  match p with
+  | [] -> []
+  | Tau_choice :: p -> ipos_trace p
+  | Call_choice o x y :: p -> Call_choice o x y :: ipos_trace p
+
+let rec ipos_trace_append (p q : iopos) :
+  Lemma (ensures ipos_trace (p @ q) == ipos_trace p @ ipos_trace q) (decreases p)
+= match p with
+  | [] -> ()
+  | Tau_choice :: p -> ipos_trace_append p q
+  | Call_choice o x y :: p -> ipos_trace_append p q
+
+noeq
+type branch a =
+| Fin : tr:trace -> res:a -> branch a
+| Inf : p : iopostream -> branch a
+
+unfold
+let wpost a = branch a -> Type0
+
+let twp a = wpost a -> Type0
+
+let wret #a (x : a) : twp a =
+  fun post -> post (Fin [] x)
+
+let rec trace_to_pos (tr : trace) : iopos =
+  match tr with
+  | [] -> []
+    | c :: tr -> c :: trace_to_pos tr
+
+let shift_post #a (tr : trace) (post : wpost a) : wpost a =
+  fun b ->
+    match b with
+    | Fin tr' x -> post (Fin (tr @ tr') x)
+    | Inf p -> post (Inf (postream_prepend (trace_to_pos tr) p))
+
+let wbind #a #b (w : twp a) (wf : a -> twp b) : twp b =
+  fun post ->
+    w (fun b ->
+      match b with
+      | Fin tr x -> wf x (shift_post tr post)
+      | Inf p -> post (Inf p)
+    )
+
+let stronger_twp #a (wp1 wp2 : twp a) : Type0 =
+  forall post. wp1 post ==> wp2 post
+
+(** Effect observation *)
+let theta #a (t : iotree a) =
+  fun post ->
+    (forall p. isRet (t p) ==> post (Fin (ipos_trace p) (ret_val (t p)))) /\
+    (forall (p : iopostream).
+      (forall n. isEvent (t (postream_trunc p n))) ==>
+      post (Inf p)
+    )
+
+let iodiv a (w : twp a) =
+  t: iotree a { w `stronger_twp` theta t }
+
+let iodiv_ret a (x : a) : iodiv a (wret x) =
+  assert (forall p. ~ (isEvent (ioret x p))) ;
+  assert (forall (p : iopostream). ~ (isEvent (ioret x (postream_trunc p 0)))) ;
+  ret x
+
+// let iodiv_bind a b w wf (m : iodiv a w) (f : (x:a) -> iodiv b (wf x)) : iodiv b (wbind w wf) =
+//   assert (forall (post : wpost a). w post ==> theta m post) ;
+//   assert (forall (post : wpost b) x. wf x post ==> theta (f x) post) ;
+
+//   // ret
+//   forall_intro (find_ret_Some_pos m []) ;
+//   forall_intro_2 ipos_trace_append ;
+//   forall_intro (find_ret_prefix_val m []) ;
+//   assert (forall (post : wpost b) p. wbind w wf post ==> isRet (bind m f p) ==> post (ipos_trace p) (Some (ret_val (bind m f p)))) ;
+
+//   // event.ret
+//   assert (forall (post : wpost b) p. wbind w wf post ==> isEvent (bind m f p) ==> Some? (find_ret m [] p) ==> post (ipos_trace p) None) ;
+
+//   // event.noret
+//   assert (forall (post : wpost b) p.
+//     wbind w wf post ==>
+//     isEvent (bind m f p) ==>
+//     None? (find_ret m [] p) ==>
+//     isEvent (m p)
+//   ) ;
+//   assert (forall (post : wpost b) p. wbind w wf post ==> isEvent (bind m f p) ==> None? (find_ret m [] p) ==> post (ipos_trace p) None) ;
+
+//   // event
+//   assert (forall (post : wpost b) p. wbind w wf post ==> isEvent (bind m f p) ==> post (ipos_trace p) None) ;
+
+//   assert (forall (post : wpost b). wbind w wf post ==> theta (bind m f) post) ;
+//   bind m f
+
+// let twp_tau #a (w : twp a) : twp a =
+//   fun post -> post [] None /\ w post
+
+// let iodiv_tau #a #w (m : iodiv a w) : iodiv a (twp_tau w) =
+//   tau m
+
+// let twp_call #a (o : cmds) (x : io_args o) (w : io_res o -> twp a) : twp a =
+//   fun post -> post [] None /\ (forall y. w y (shift_post [ Call_choice o x y ] post))
+
+// let iodiv_call #a (o : cmds) (x : io_args o) #w (k : (r : io_res o) -> iodiv a (w r)) : iodiv a (twp_call o x w) =
+//   call o x k
+
+// let rec twp_repeat_trunc (w : twp unit) (n : nat) : twp unit =
+//   if n = 0
+//   then fun post -> True
+//   else wbind w (fun (_:unit) -> twp_tau (twp_repeat_trunc w (n - 1)))
+
+// let twp_repeat (w : twp unit) : twp unit =
+//   fun post -> forall n. twp_repeat_trunc w n post
+
+// let repeat_unfold_1 (body : iotree unit) :
+//   Lemma (forall p. repeat body p == bind body (fun _ -> tau ((if length p = 0 then (fun _ -> loop _) else itree_cofix_unfoldn (repeat_fix body) (length p - 1)) ())) p)
+// = forall_intro (itree_cofix_unfold_1 (repeat_fix body) ()) ;
+//   forall_intro_2 (repeat_fix_guarded body) ;
+//   assert (forall p. itree_cofix (repeat_fix body) () p == repeat_fix body (if length p = 0 then (fun _ -> loop _) else itree_cofix_unfoldn (repeat_fix body) (length p - 1)) () p) ;
+//   assert (forall p. itree_cofix (repeat_fix body) () p == bind body (fun _ -> tau ((if length p = 0 then (fun _ -> loop _) else itree_cofix_unfoldn (repeat_fix body) (length p - 1)) ())) p)
+
+// let repeat_one_ret (body : iotree unit) :
+//   Lemma (forall p q. isRet (body p) ==> repeat body (p @ Tau_choice :: q) == repeat body q)
+// = repeat_unfold_1 body ;
+//   find_ret_append body ;
+//   assert (forall p q.
+//     isRet (body p) ==>
+//     repeat body (p @ Tau_choice :: q) == itree_cofix_unfoldn (repeat_fix body) (length (p @ Tau_choice :: q) - 1) () q
+//   ) ;
+//   forall_intro_2 (repeat_fix_guarded body)
+
+// let rec repeat_not_ret (body : iotree unit) p :
+//   Lemma (~ (isRet (repeat body p)))
+// = match find_ret body [] p with
+//   | Some ((), q) ->
+//     repeat_unfold_1 body ;
+//     if length p = 0
+//     then ()
+//     else begin
+//       match q with
+//       | Tau_choice :: r ->
+//         find_ret_length body [] p ;
+//         forall_intro_2 (repeat_fix_guarded body) ;
+//         find_ret_smaller body [] p ;
+//         repeat_not_ret body r
+//       | _ :: r -> ()
+//       | [] -> ()
+//     end
+//   | None -> ()
+
+// let rec repeat_any_ret (body : iotree unit) (pl : list iopos) p :
+//   Lemma
+//     (requires forall pp. mem pp pl ==> isRet (body pp))
+//     (ensures repeat body (flatten_sep [Tau_choice] pl @ p) == repeat body p)
+// = match pl with
+//   | [] -> ()
+//   | pp :: pl ->
+//     calc (==) {
+//       repeat body (flatten_sep [Tau_choice] (pp :: pl) @ p) ;
+//       == {}
+//       repeat body ((pp @ [Tau_choice] @ flatten_sep [Tau_choice] pl) @ p) ;
+//       == { forall_intro_3 (append_assoc #iochoice) }
+//       repeat body (pp @ Tau_choice :: (flatten_sep [Tau_choice] pl @ p)) ;
+//       == { repeat_one_ret body }
+//       repeat body (flatten_sep [Tau_choice] pl @ p) ;
+//       == { repeat_any_ret body pl p }
+//       repeat body p ;
+//     }
+
+// let rec repeat_any_ret_event_post #w (body : iodiv unit w) (pl : list iopos) p :
+//   Lemma
+//     (requires forall pp. mem pp pl ==> isRet (body pp))
+//     (ensures forall (post : wpost unit).
+//       twp_repeat_trunc w (1 + length pl) post ==>
+//       isEvent (body p) ==>
+//       post (ipos_trace (flatten_sep [Tau_choice] pl @ p)) None
+//     )
+//     (decreases pl)
+// = match pl with
+//   | [] -> ()
+//   | pp :: pl ->
+//     repeat_any_ret_event_post body pl p ;
+//     calc (==) {
+//       ipos_trace (flatten_sep [Tau_choice] (pp :: pl) @ p) ;
+//       == {}
+//       ipos_trace ((pp @ Tau_choice :: flatten_sep [Tau_choice] pl) @ p) ;
+//       == { forall_intro_3 (append_assoc #iochoice) }
+//       ipos_trace (pp @ Tau_choice :: flatten_sep [Tau_choice] pl @ p) ;
+//       == { forall_intro_2 ipos_trace_append }
+//       ipos_trace pp @ ipos_trace (Tau_choice :: flatten_sep [Tau_choice] pl @ p) ;
+//       == {}
+//       ipos_trace pp @ ipos_trace (flatten_sep [Tau_choice] pl @ p) ;
+//     }
+
+// let rec repeat_any_ret_ret_post #w (body : iodiv unit w) (pl : list iopos) p :
+//   Lemma
+//     (requires forall pp. mem pp pl ==> isRet (body pp))
+//     (ensures forall (post : wpost unit).
+//       twp_repeat_trunc w (1 + length pl) post ==>
+//       isRet (body p) ==>
+//       post (ipos_trace (flatten_sep [Tau_choice] pl @ p)) None
+//     )
+//     (decreases pl)
+// = match pl with
+//   | [] ->
+//     assert (forall (post : wpost unit).
+//       twp_repeat_trunc w 1 post ==>
+//       isRet (body p) ==>
+//       twp_tau (twp_repeat_trunc w 0) (shift_post (ipos_trace p) post)
+//     )
+//   | pp :: pl ->
+//     repeat_any_ret_ret_post body pl p ;
+//     assert (forall (post : wpost unit).
+//       twp_repeat_trunc w (1 + length pl) post ==>
+//       isRet (body p) ==>
+//       post (ipos_trace (flatten_sep [Tau_choice] pl @ p)) None
+//     ) ;
+//     assert (forall (post : wpost unit).
+//       twp_repeat_trunc w (1 + length pl) (shift_post (ipos_trace pp) post) ==>
+//       isRet (body p) ==>
+//       shift_post (ipos_trace pp) post (ipos_trace (flatten_sep [Tau_choice] pl @ p)) None
+//     ) ;
+//     calc (==) {
+//       ipos_trace (flatten_sep [Tau_choice] (pp :: pl) @ p) ;
+//       == {}
+//       ipos_trace ((pp @ Tau_choice :: flatten_sep [Tau_choice] pl) @ p) ;
+//       == { forall_intro_3 (append_assoc #iochoice) }
+//       ipos_trace (pp @ Tau_choice :: flatten_sep [Tau_choice] pl @ p) ;
+//       == { forall_intro_2 ipos_trace_append }
+//       ipos_trace pp @ ipos_trace (Tau_choice :: flatten_sep [Tau_choice] pl @ p) ;
+//       == {}
+//       ipos_trace pp @ ipos_trace (flatten_sep [Tau_choice] pl @ p) ;
+//     } ;
+//     assert (forall (post : wpost unit).
+//       twp_repeat_trunc w (1 + length pl) (shift_post (ipos_trace pp) post) ==>
+//       isRet (body p) ==>
+//       post (ipos_trace (flatten_sep [Tau_choice] (pp :: pl) @ p)) None
+//     ) ;
+//     assert (forall (post : wpost unit).
+//       twp_repeat_trunc w (2 + length pl) post ==>
+//       isRet (body p) ==>
+//       post (ipos_trace (flatten_sep [Tau_choice] (pp :: pl) @ p)) None
+//     )
+
+// let rec iodiv_repeat_proof_gen #w (body : iodiv unit w) (pl : list iopos) p :
+//   Lemma
+//     (requires forall pp. mem pp pl ==> isRet (body pp))
+//     (ensures forall (post : wpost unit).
+//       twp_repeat w post ==>
+//       isEvent (repeat body (flatten_sep [Tau_choice] pl @ p)) ==>
+//       post (ipos_trace (flatten_sep [Tau_choice] pl @ p)) None
+//     )
+//     (decreases p)
+// = match find_ret body [] p with
+//   | Some ((), q) ->
+//     assert (isRet (body (find_ret_prefix body [] p))) ;
+//     find_ret_Some_pos body [] p ;
+//     assert (p == find_ret_prefix body [] p @ q) ;
+//     begin match q with
+//     | [] ->
+//       repeat_any_ret body pl p ;
+//       repeat_unfold_1 body ;
+//       assert (repeat body p == Some Tau) ;
+//       repeat_any_ret_ret_post body pl p ;
+//       assert (isRet (body p)) ;
+//       assert (forall (post : wpost unit). twp_repeat w post ==> twp_repeat_trunc w (1 + length pl) post) ;
+//       assert (forall (post : wpost unit).
+//         twp_repeat w post ==>
+//         isEvent (repeat body p) ==>
+//         post (ipos_trace (flatten_sep [Tau_choice] pl @ p)) None
+//       )
+//     | Tau_choice :: r ->
+//       forall_intro (mem_append pl [find_ret_prefix body [] p]) ;
+//       assert (forall pp. mem pp (pl @ [find_ret_prefix body [] p]) ==> isRet (body pp)) ;
+//       assert (p == find_ret_prefix body [] p @ Tau_choice :: r) ;
+//       forall_intro_3 (append_assoc #iochoice) ;
+//       forall_intro_2 (flatten_sep_append #iochoice [Tau_choice]) ;
+//       assert (flatten_sep [Tau_choice] (pl @ [find_ret_prefix body [] p]) == flatten_sep [Tau_choice] pl @ flatten_sep [Tau_choice] [find_ret_prefix body [] p]) ;
+//       assert (flatten_sep [Tau_choice] [find_ret_prefix body [] p] == find_ret_prefix body [] p @ [Tau_choice] @ flatten_sep [Tau_choice] []) ;
+//       flatten_sep_nil #iochoice [Tau_choice] ;
+//       assert (flatten_sep [Tau_choice] pl @ p == flatten_sep [Tau_choice] (pl @ [find_ret_prefix body [] p]) @ r) ;
+//       find_ret_smaller body [] p ;
+//       iodiv_repeat_proof_gen body (pl @ [find_ret_prefix body [] p]) r
+//     | c :: r -> repeat_any_ret body pl p ; repeat_unfold_1 body
+//     end
+//   | None ->
+//     repeat_any_ret body pl p ;
+//     repeat_any_ret_event_post body pl p ;
+//     assert (forall (post : wpost unit). twp_repeat w post ==> twp_repeat_trunc w (1 + length pl) post) ;
+//     repeat_unfold_1 body ;
+//     assert (
+//       isEvent (repeat body p) ==> isEvent (body p)
+//     ) ;
+//     assert (forall (post : wpost unit).
+//       twp_repeat w post ==>
+//       isEvent (repeat body p) ==>
+//       post (ipos_trace (flatten_sep [Tau_choice] pl @ p)) None
+//     )
+
+// let iodiv_repeat_proof #w (body : iodiv unit w) p :
+//   Lemma (forall (post : wpost unit).
+//     twp_repeat w post ==>
+//     isEvent (repeat body p) ==>
+//     post (ipos_trace p) None
+//   )
+// = iodiv_repeat_proof_gen body [] p
+
+// let iodiv_repeat #w (body : iodiv unit w) : iodiv unit (twp_repeat w) =
+//   forall_intro (repeat_not_ret body) ;
+//   forall_intro (iodiv_repeat_proof body) ;
+//   repeat body
+
+// // We can also "inline" the induction by asking the SMT to prove (p n ==> p (n+1)) which might work sometimes
+
+// (**
+
+//   Alternatively, we propose a definition of iodiv_repeat using an invariant.
+//   The invariant is relative to the predicate transformer of the body.
+//   It must hold for the empty list / root position because postconditions
+//   must be downward closed.
+
+// *)
+
+// let trace_invariant (w : twp unit) (inv : trace -> Type0) =
+//   inv [] /\
+//   (forall tr. inv tr ==> w (fun tr' v -> inv (tr @ tr') /\ Some? v))
+
+// let twp_repeat_with_inv (w : twp unit) (inv : trace -> Type0) : twp unit =
+//   fun post -> forall tr. inv tr ==> post tr None
+
+// let invpost (inv : trace -> Type0) : wpost unit =
+//   fun tr v -> inv tr /\ None? v
+
+// // Maybe prove it on the effect observation directly
+// let rec twp_repeat_inv_trunc (w : twp unit) (inv : trace -> Type0) n :
+//   Lemma (
+//     trace_invariant w inv ==>
+//     twp_repeat_trunc w n (invpost inv)
+//   )
+// = if n = 0
+//   then ()
+//   else begin
+//     twp_repeat_inv_trunc w inv (n - 1) ;
+//     assume (
+//       trace_invariant w inv ==>
+//       twp_repeat_trunc w (n-1) (invpost inv) ==>
+//       wbind w (fun (_:unit) -> twp_tau (twp_repeat_trunc w (n - 1))) (invpost inv)
+//       // ==
+//       // w (fun tr v ->
+//       //   match v with
+//       //   | Some x -> (fun (_:unit) -> twp_tau (twp_repeat_trunc w (n - 1))) x (shift_post tr (invpost inv))
+//       //     == twp_tau (twp_repeat_trunc w (n - 1)) (shift_post tr (invpost inv))
+//       //   | None -> invpost inv tr None // == inv tr
+//       // )
+//     ) ;
+//     assume (forall (post : wpost unit).
+//       wbind w (fun (_:unit) -> twp_tau (twp_repeat_trunc w (n - 1))) post ==>
+//       twp_repeat_trunc w n post
+//     ) ; // why??
+//     assert (
+//       trace_invariant w inv ==>
+//       twp_repeat_trunc w (n-1) (invpost inv) ==>
+//       twp_repeat_trunc w n (invpost inv)
+//     )
+//   end
+
+// // Some specifications
+
+// // Does not make sense at the moment
+// // let terminates #a : wpost a =
+// //   fun tr v -> Some? v
+
+// let diverges #a : wpost a =
+//   fun tr v -> None? v
+
+// // let ret_terminates a (x : a) : Lemma (wret x terminates) = ()
+
+// // Should be p1 ==> p2 rather than ==
+// let rec twp_repeat_trunc_ext w n (p1 p2 : wpost unit) :
+//   Lemma ((forall tr x. p1 tr x == p2 tr x) ==> twp_repeat_trunc w n p1 == twp_repeat_trunc w n p2)
+// = if n = 0
+//   then ()
+//   else begin
+//     // twp_repeat_trunc_ext w (n-1) p1 p2 ;
+//     // assume ((forall tr x. p1 tr x == p2 tr x) ==> wbind w (fun _ -> twp_repeat_trunc w (n -1)) p1 == wbind w (fun _ -> twp_repeat_trunc w (n -1)) p2)
+//     // assert (twp_repeat_trunc w n == wbind w (fun _ -> twp_repeat_trunc w (n -1))) ; // Isn't this by def??
+//     assume ((forall tr x. p1 tr x == p2 tr x) ==> twp_repeat_trunc w n p1 == twp_repeat_trunc w n p2)
+//   end
+
+// let repeat_ret_loops () :
+//   Lemma (twp_repeat (wret ()) diverges)
+// = let rec aux n :
+//     Lemma (twp_repeat_trunc (wret ()) n diverges) [SMTPat ()]
+//   = if n = 0
+//     then ()
+//     else begin
+//       aux (n - 1) ;
+//       twp_repeat_trunc_ext (wret ()) (n-1) (shift_post [] diverges) (diverges #unit)
+//     end
+//   in
+//   ()
+
+// // Much better
+// let repeat_ret_loops_with_inv () :
+//   Lemma (twp_repeat_with_inv (wret ()) (fun _ -> True) diverges)
+// = ()
+
+// [@@allow_informative_binders]
+// reifiable total layered_effect {
+//   IODiv : a:Type -> twp a -> Effect
+//   with
+//     repr   = iodiv ;
+//     return = iodiv_ret ;
+//     bind   = iodiv_bind
+//     // tau    = iodiv_tau ; // Universe problems
+//     // call   = iodiv_call
+// }
